src/program_proof/unittest.v
@@ -1,0 +1,19 @@
+From Perennial.program_proof Require Import disk_prelude.
+From Goose.github_com.tchajed.goose Require Import unittest.
+
+Section proof.
+Context `{!heapGS Σ}.
+
+Lemma proph_test : ⊢ WP unittest.Oracle #() {{ _, True }}.
+Proof.
+  wp_lam.
+  wp_apply wp_NewProph_list.
+  iIntros (pvs p) "Hp".
+  wp_apply (wp_ResolveProph_list with "Hp").
+  iIntros (pvs') "[_ Hp]".
+  wp_apply (wp_ResolveProph_list with "Hp").
+  iIntros (pvs'') "[_ Hp]".
+  wp_pures. auto.
+Qed.
+
+End proof.
